nr: introduce tracking of already read bits
in the end when we bump the local tail, we must have read
everything between the old and new local tail. this implies
that all entries in between must have been alive. This
change introduces a "current" pointer in the Reader state
that tracks which entry is the next to be read.

Signed-off-by: Reto Achermann <achreto@gmail.com>

concurrency/node-replication/CyclicBuffer.i.dfy
@@ -24,7 +24,7 @@ module CyclicBufferRw(nrifc: NRIfc) refines MultiRw {
 
   datatype ReaderState =
     | ReaderStarting(ghost start: nat)
-    | ReaderRange(ghost start: nat, ghost end: nat)
+    | ReaderRange(ghost start: nat, ghost end: nat, ghost cur: nat)
     | ReaderGuard(ghost start: nat, ghost end: nat, ghost cur: nat, ghost val: StoredType)
 
   datatype CombinerState =
@@ -207,13 +207,19 @@ module CyclicBufferRw(nrifc: NRIfc) refines MultiRw {
           // the starting value should match the local tail
           && start == x.localTails[n]
         )
-        case ReaderRange(start: nat, end: nat) => (
+        case ReaderRange(start: nat, end: nat, cur: nat) => (
           // the start must be our local tail
           && x.localTails[n] == start
           // the start must be before the end, can be equial if ltail == gtail
           && start <= end
           // we've read the tail, but the tail may have moved
           && x.tail.value - (BUFFER_SIZE as nat) <= end <= x.tail.value
+          // current is between start and end
+          && start <= cur <= end
+          // the entries up to, and including  current must be alive
+          && (forall i | start <= i < cur :: EntryIsAlive(x.aliveBits, i))
+          // the entries up to, and including current must have something in the log
+          && (forall i | start <= i < cur :: x.contents[i].Some?)
         )
         case ReaderGuard(start: nat, end: nat, cur: nat, val: StoredType) => (
           // the start must be our local tail
@@ -224,8 +230,10 @@ module CyclicBufferRw(nrifc: NRIfc) refines MultiRw {
           && x.tail.value - (BUFFER_SIZE as nat) <= end <= x.tail.value
           // current is between start and end
           && start <= cur < end
-          // the entry that we read must be alive
-          && EntryIsAlive(x.aliveBits, cur)
+          // the entries up to, and including  current must be alive
+          && (forall i | start <= i <= cur :: EntryIsAlive(x.aliveBits, i))
+          // the entries up to, and including current must have something in the log
+          && (forall i | start <= i <= cur :: x.contents[i].Some?)
           // the thing we are ready should match the log content
           && x.contents[cur] == Some(val)
         )
@@ -272,7 +280,7 @@ module CyclicBufferRw(nrifc: NRIfc) refines MultiRw {
       case CombinerReading(readerState: ReaderState) => (
         match readerState {
           case ReaderStarting(_) => {}
-          case ReaderRange(start: nat, end: nat) => {} // not really accessing yet
+          case ReaderRange(start: nat, end: nat, _) => {} // not really accessing yet
           case ReaderGuard(start: nat, end: nat, cur: nat , _) => (
             {cur} // we only access this one.
           )
@@ -330,11 +338,11 @@ module CyclicBufferRw(nrifc: NRIfc) refines MultiRw {
     && Complete(x)
     && PointerOrdering(x)
     && PointerDifferences(x)
+    && RangesNoOverlap(x)
     && AliveBits(x)
     && BufferContents(x)
     // let's use the non-set version
     // && LogicalRangesNoOverlap(x)
-    && RangesNoOverlap(x)
     && CombinerStateValid(x)
     && ReaderStateValid(x)
   }
@@ -638,13 +646,7 @@ module CyclicBufferRw(nrifc: NRIfc) refines MultiRw {
   {
     && m.combinerState[nodeId].CombinerReading?
     && m.combinerState[nodeId].readerState.ReaderRange?
-  }
-
-  predicate CombinerIsReaderRangeAt(m: M, nodeId: NodeId, start: nat, end: nat)
-    requires m.M?
-    requires CombinerKnown(m, nodeId)
-  {
-    && m.combinerState[nodeId] == CombinerReading(ReaderRange(start, end))
+    && m.combinerState[nodeId].readerState.cur < m.combinerState[nodeId].readerState.end
   }
 
   predicate CombinerIsReaderGuard(m: M, nodeId: NodeId)
@@ -653,6 +655,15 @@ module CyclicBufferRw(nrifc: NRIfc) refines MultiRw {
   {
     && m.combinerState[nodeId].CombinerReading?
     && m.combinerState[nodeId].readerState.ReaderGuard?
+  }
+
+  predicate CombinerIsReaderRangeDone(m: M, nodeId: NodeId)
+    requires m.M?
+    requires CombinerKnown(m, nodeId)
+  {
+    && m.combinerState[nodeId].CombinerReading?
+    && m.combinerState[nodeId].readerState.ReaderRange?
+    && m.combinerState[nodeId].readerState.cur == m.combinerState[nodeId].readerState.end
   }
 
   /*
@@ -865,13 +876,13 @@ module CyclicBufferRw(nrifc: NRIfc) refines MultiRw {
       contents := m.contents[key := Some(deposited)])
   }
 
+  // seems to take about 4 minutes...
   lemma AppendFlipBit_is_deposit(m: M, m': M, combinerNodeId: nat, deposited: StoredType)
-  requires AppendFlipBit(m, m', combinerNodeId, deposited)
-  ensures exists key :: deposit(m, m', key, deposited)
+    requires AppendFlipBit(m, m', combinerNodeId, deposited)
+    ensures exists key :: deposit(m, m', key, deposited)
   {
     var combinerBefore := m.combinerState[combinerNodeId];
     var key := combinerBefore.cur_idx;
-    var tail := combinerBefore.tail;
 
     forall p: M | Inv(dot(m, p))
     ensures Inv(dot(m', p))
@@ -888,7 +899,10 @@ module CyclicBufferRw(nrifc: NRIfc) refines MultiRw {
             (&& EntryIsAlive(dot(m', p).aliveBits, i) == EntryIsAlive(dot(m, p).aliveBits, i)
             && !EntryIsAlive(dot(m', p).aliveBits, i))
           );
-       }
+      }
+
+      assert AliveBits(dot(m', p));
+      assert BufferContents(dot(m', p));
 
       assert Inv(dot(m', p));
       assert key !in I(dot(m, p));
@@ -942,7 +956,7 @@ module CyclicBufferRw(nrifc: NRIfc) refines MultiRw {
     && var readerBefore := m.combinerState[combinerNodeId].readerState;
 
     && m' == m.(combinerState := m.combinerState[combinerNodeId := CombinerReading(
-      ReaderRange(readerBefore.start, m.tail.value))]
+      ReaderRange(readerBefore.start, m.tail.value, readerBefore.start))]
     )
   }
 
@@ -971,7 +985,12 @@ module CyclicBufferRw(nrifc: NRIfc) refines MultiRw {
 
     && i in m.contents
     && m.contents[i].Some?
-    && readerBefore.start <= i < readerBefore.end
+    // Question(RA): we sort of require to  process all entries before completing
+    //               and updating the local tail value. right now this is done
+    //               using the cur pointer, and requires linear processing of
+    //               the log, not sure if this causes a problem somewhere.
+    // && readerBefore.start <= i < readerBefore.end
+    && readerBefore.cur == i
 
     && LogicalToPhysicalIndex(i) in m.aliveBits
     && EntryIsAlive(m.aliveBits, i)
@@ -1007,7 +1026,7 @@ module CyclicBufferRw(nrifc: NRIfc) refines MultiRw {
 
     && m' == m.(
       combinerState := m.combinerState[combinerNodeId := CombinerReading(
-        ReaderRange(readerBefore.start, readerBefore.end))]
+        ReaderRange(readerBefore.start, readerBefore.end, readerBefore.cur + 1))]
     )
   }
 
@@ -1031,7 +1050,7 @@ module CyclicBufferRw(nrifc: NRIfc) refines MultiRw {
     && m.M?
 
     && CombinerKnown(m, combinerNodeId)
-    && CombinerIsReaderRange(m, combinerNodeId)
+    && CombinerIsReaderRangeDone(m, combinerNodeId)
     && var combinerBefore := m.combinerState[combinerNodeId];
     && var readerBefore := m.combinerState[combinerNodeId].readerState;
 
@@ -1051,14 +1070,19 @@ module CyclicBufferRw(nrifc: NRIfc) refines MultiRw {
     ensures Inv(dot(m', p))
       && I(dot(m, p)) == I(dot(m', p))
     {
-      if MinLocalTail(dot(m', p).localTails) == MinLocalTail(dot(m, p).localTails) {
+      if MinLocalTail(dot(m, p).localTails) == MinLocalTail(dot(m', p).localTails) {
         assert Inv(dot(m', p));
         assert I(dot(m, p)) == I(dot(m', p));
       } else {
-        assume MinLocalTail(dot(m', p).localTails) > MinLocalTail(dot(m, p).localTails);
+        assert MinLocalTail(dot(m, p).localTails) < MinLocalTail(dot(m', p).localTails);
+        var old_mintails := MinLocalTail(dot(m, p).localTails);
+        var new_mintails := MinLocalTail(dot(m', p).localTails);
 
-        assume AliveBits(dot(m', p)); // fails
-        assume BufferContents(dot(m', p)); // fails
+        // everything between old_mintails and new_mintails had to be alive, otherwise we
+        // couldn't have processed it. Now, transform this into the !Alive for the new mintail
+        assert forall i | old_mintails <= i < new_mintails :: EntryIsAlive(dot(m', p).aliveBits, i);
+        EntryIsAliveWrapAround(dot(m', p).aliveBits, old_mintails , new_mintails );
+        EntryIsAliveWrapAroundReformat(dot(m', p).aliveBits, old_mintails , new_mintails );
 
         assert Inv(dot(m', p));
         assert I(dot(m, p)) == I(dot(m', p));
